Refactored quicksorts. Proved a lemma relating In and count. Used it to simplify the proof of the fact that quicksort preserves In. Proved that the hybrid quicksort conforms to the specification of sorting. Greatly simplified the proof of ins_sorted. Refactored selection sorts. Tried to write a minmax variant of selection sort, but failed. Simplified proof of the lemma ss_In.

Sorting/HybridSorts.v
@@ -6,19 +6,3 @@ Require Import QuickSort.
 Require Import MergeSort.
 
 Set Implicit Arguments.
-
-Function hqs (A : LinDec) (n : nat) (l : list A) {measure length l} : list A :=
-  if @leqb natle (length l) n
-  then insertionSort A l
-  else match l with
-      | [] => []
-      | h :: t =>
-          let (lo, hi) := bifilter (fun x : A => x <=? h) t in
-              hqs A n lo ++ h :: hqs A n hi
-  end.
-Proof.
-  intros. rewrite bifilter_spec in teq1. inversion teq1.
-    apply filter_lengthOrder.
-  intros. rewrite bifilter_spec in teq1. inversion teq1.
-    apply filter_lengthOrder.
-Defined.
