Sorting/QuickSort.v
@@ -6,133 +6,29 @@ Require Export Recdef.
 Require Export Sort.
 Require Export ListLemmas.
 
+Require Import InsertionSort.
+
 Set Implicit Arguments.
 
-Hint Resolve le_n_S filter_length.
-
-(* Quicksort using Program Fixpoint *)
-Program Fixpoint qsPF (A : LinDec) (l : list A) {measure (length l)}
-    : list A :=
-match l with
-    | [] => []
-    | h :: t => qsPF A (filter (fun x : A => leqb x h) t) ++ [h]
-             ++ qsPF A (filter (fun x : A => negb (leqb x h)) t)
-end.
-Next Obligation. simpl. unfold lt. auto. Qed.
-Next Obligation. simpl. unfold lt. auto. Qed.
-
-Eval compute in qsPF natle testl.
+Local Hint Unfold lt.
+Local Hint Resolve le_n_S filter_length.
 
 (* Quicksort using Function. *)
-Function qsFun (A : LinDec) (l : list A) {measure length l} : list A :=
+Function qs (A : LinDec) (l : list A) {measure length l} : list A :=
 match l with
     | [] => []
-    | h :: t => qsFun A (filter (fun x : A => leqb x h) t) ++
-           h :: qsFun A (filter (fun x : A => negb (leqb x h)) t)
+    | h :: t => qs A (filter (fun x : A => leqb x h) t) ++
+           h :: qs A (filter (fun x : A => negb (leqb x h)) t)
 end.
-Proof.
-  intros. unfold lt. simpl. apply le_n_S. apply filter_length.
-  intros. unfold lt. simpl. apply le_n_S. apply filter_length.
-Defined.
+Proof. all: simpl; auto. Defined.
 
-Eval compute in qsFun natle testl.
+Eval compute in qs natle testl.
 
-(* Quicksort using fuel recursion. *)
-Fixpoint qsFuel' (A : LinDec) (fuel : nat) (l : list A) : list A :=
-match fuel, l with
-    | 0, _ => l
-    | _, [] => []
-    | _, [x] => [x]
-    | S fuel', h :: t =>
-        qsFuel' A fuel' (filter (fun x : A => leqb x h) t) ++ h ::
-        qsFuel' A fuel' (filter (fun x : A => negb (leqb x h)) t)
+Local Hint Extern 0 (length _ < length _) =>
+match goal with
+    | H : bifilter _ _ = _ |- _ => rewrite bifilter_spec in H; inversion H;
+        apply filter_lengthOrder
 end.
-
-Definition qsFuel (A : LinDec) (l : list A) : list A :=
-    qsFuel' A (length l) l.
-
-Eval compute in (qsFuel natle testl).
-
-(* Quicksort using well-founded recursion. *)
-Definition qsWf (A : LinDec) : list A -> list A.
-Proof.
-  apply (Fix (@lengthOrder_wf A) _).
-  intros l qsWf.
-  destruct l as [| h t].
-    exact [].
-    pose (le := qsWf (filter (fun x : A => leqb x h) t)
-        (filter_lengthOrder (fun x => leqb x h) h t)).
-    pose (gt := qsWf (filter (fun x : A => negb (leqb x h)) t)
-        (filter_lengthOrder (fun x : A => negb (leqb x h)) h t)).
-    exact (le ++ h :: gt).
-Defined.
-
-Eval compute in qsWf natle testl.
-
-(* Quicksort using wel-founded recursion and refine. *)
-Definition qsWfRef (A : LinDec) : list A -> list A.
-refine (Fix (@lengthOrder_wf A) _ (fun (l : list A) =>
-match l with
-    | [] => fun _ => []
-    | h :: t => fun qs =>
-        qs (filter (fun x : A => leqb x h) t) _ ++ h ::
-        qs (filter (fun x : A => negb (leqb x h)) t) _
-end)).
-Proof.
-  apply filter_lengthOrder.
-  apply filter_lengthOrder.
-Defined.
-
-Eval compute in qsWfRef natle testl.
-
-(* Quicksort using Bove-Capretta *)
-Inductive qsDom {A : LinDec} : list A -> Type :=
-    | qsDom0 : qsDom nil
-    | qsDom1 : forall (h : A) (t : list A),
-        qsDom (filter (fun x : A => leqb x h) t) ->
-        qsDom (filter (fun x : A => negb (leqb x h)) t) ->
-        qsDom (h :: t).
-
-Fixpoint qsBC' {A : LinDec} (l : list A) (dom : qsDom l) : list A :=
-match dom with
-    | qsDom0 => nil
-    | qsDom1 h t dom1 dom2 =>
-        qsBC' dom1 ++ h :: qsBC' dom2
-end.
-
-Theorem all_qsDom : forall (A : LinDec) (l : list A), qsDom l.
-Proof.
-  intro. apply well_founded_induction_type with lengthOrder.
-    apply lengthOrder_wf.
-    intros. destruct x as [| h t]; constructor; apply X.
-      simpl. unfold lt. apply le_n_S. apply filter_length.
-      simpl. unfold lt. apply le_n_S. apply filter_length.
-Defined.
-
-Definition qsBC (A : LinDec) (l : list A) : list A :=
-    @qsBC' A l (all_qsDom A l).
-
-Eval compute in qsBC natle testl.
-
-(* Now the serious part. TODO *)
-Definition qs := qsFun.
-
-Function bifilter {A : Type} (p : A -> bool) (l : list A)
-    : list A * list A :=
-match l with
-    | [] => ([], [])
-    | h :: t =>
-        let (l1, l2) := bifilter p t in
-        if p h then (h :: l1, l2) else (l1, h :: l2)
-end.
-
-Theorem bifilter_spec :
-  forall (A : Type) (p : A -> bool) (l : list A),
-    bifilter p l = (filter p l, filter (fun x : A => negb (p x)) l).
-Proof.
-  intros. functional induction @bifilter A p l; simpl;
-  rewrite ?e1; simpl; try rewrite e0 in IHp0; try inversion IHp0; auto.
-Qed.
 
 Function qs2 (A : LinDec) (l : list A) {measure length l} : list A :=
 match l with
@@ -141,49 +37,7 @@ match l with
         let (lo, hi) := bifilter (fun x : A => x <=? h) t in
         qs2 A lo ++ h :: qs2 A hi
 end.
-Proof.
-  intros. rewrite bifilter_spec in teq0. inversion teq0.
-    apply filter_lengthOrder.
-  intros. rewrite bifilter_spec in teq0. inversion teq0.
-    apply filter_lengthOrder.
-Defined.
-
-Theorem qs2_is_qs :
-  forall (A : LinDec) (l : list A), qs2 A l = qs A l.
-Proof.
-  intros. functional induction qs2 A l.
-    compute. trivial.
-    unfold qs. rewrite qsFun_equation. rewrite bifilter_spec in e0.
-      inversion e0. rewrite H0, H1. repeat f_equal; auto.
-Qed.
-
-Function trifilter (A : LinDec) (pivot : A) (l : list A)
-  : list A * list A * list A :=
-match l with
-    | [] => ([], [], [])
-    | h :: t =>
-        let '(l1, l2, l3) := trifilter A pivot t in
-        if h <=? pivot
-        then if pivot <=? h then (l1, h :: l2, l3) else (h :: l1, l2, l3)
-        else (l1, l2, h :: l3)
-end.
-
-Compute trifilter natle 5 [1; 5; 5; 5; 2].
-
-Theorem trifilter_spec :
-  forall (A : LinDec) (pivot h : A) (t : list A),
-    trifilter A pivot (h :: t) =
-      (filter (fun x : A => x <=? pivot) (h :: t),
-       filter (fun x : A => x =? pivot) (h :: t),
-       filter (fun x : A => negb (x <=? pivot)) (h :: t)).
-Abort.
-(*  intros. rewrite trifilter_equation.
-    destruct (trifilter A pivot t) as [[l1 l2] l3].
-    Focus 2. assert (h0 = pivot) by (apply leq_antisym; auto).
-      contradiction.
-    Focus 2. contradict n. auto.
-    rewrite e0 in *. inversion IHp. rewrite <- H0, <- H1, <- H2.
-Qed.*)
+Proof. all: auto. Defined.
 
 Function qs3 (A : LinDec) (l : list A) {measure length l} : list A :=
 match l with
@@ -194,3 +48,15 @@ match l with
 end.
 Proof.
 Abort.
+
+Function hqs (n : nat) (A : LinDec) (l : list A) {measure length l}
+  : list A :=
+  if @leqb natle (length l) n
+  then insertionSort A l
+  else match l with
+      | [] => []
+      | h :: t =>
+          let (lo, hi) := bifilter (fun x : A => x <=? h) t in
+              hqs n A lo ++ h :: hqs n A hi
+  end.
+Proof. all: auto. Defined.
