Sorting/SelectionSort.v
@@ -8,156 +8,55 @@ Require Export ListLemmas.
 
 Set Implicit Arguments.
 
-(* Selection sort using program fixpoint *)
-Program Fixpoint ssPF (A : LinDec) (l : list A)
-    {measure (length l)} : list A :=
-match l with
-    | [] => []
-    | h :: t => let m := min_dflt A h t in
-        m :: ssPF A (remove_once m l)
-end.
-Next Obligation. apply remove_once_min_lengthOrder. Qed.
-
-Eval compute in ssPF natle testl.
-
 (* Selection sort using Function. *)
-Function ssFun (A : LinDec) (l : list A)
-    {wf (@lengthOrder A) l} : list A :=
+Function ss (A : LinDec) (l : list A) {measure length l} : list A :=
 match l with
     | [] => []
-    | h :: t => let m := min_dflt A h t in m :: ssFun A (remove_once m l)
+    | h :: t => let m := min_dflt A h t in m :: ss A (remove_once m l)
 end.
-Proof.
-  intros. apply remove_once_min_lengthOrder.
-  intro. apply lengthOrder_wf.
-Defined.
+Proof. intros. apply remove_once_min_lengthOrder. Defined.
 
-Eval compute in ssFun natle testl.
+Eval compute in ss natle testl.
 
-(* Selection sort using fuel recursion. *)
-Fixpoint ssFuelOpt {A : LinDec} (n : nat) (l : list A)
-    : option (list A) :=
-match n with
-    | 0 => None
-    | S n' =>
-        match l with
-            | [] => Some []
-            | h :: t => let m := min_dflt A h t in
-                match ssFuelOpt n' (remove_once m l) with
-                    | None => None
-                    | Some l' => Some (m :: l')
-                end
-            end
+Function minmax (A : LinDec) (min : A) (max : A) (l : list A) : A * A :=
+match l with
+    | [] => (min, max)
+    | h :: t =>
+        if h <=? min
+        then minmax A h max t
+        else
+          if max <=? h
+          then minmax A min h t
+          else minmax A min max t
 end.
 
-Eval compute in ssFuelOpt 15 testl.
-
-Lemma ssFuelOpt_eq : forall (A : LinDec) (n : nat) (h : A) (t : list A),
-  ssFuelOpt (S n) (h :: t) =
-    match ssFuelOpt n (remove_once (min_dflt A h t) (h :: t)) with
-        | None => None
-        | Some l => Some (min_dflt A h t :: l)
-    end.
+Lemma remove_once_In' :
+  forall (A : LinDec) (x h : A) (t : list A),
+    In x t -> x <> h -> In x (remove_once h t).
 Proof.
-  intros. reflexivity.
+  induction t as [| h' t']; cbn; intuition dec.
 Qed.
 
-Theorem ssFuelOpt_extract : forall (A : LinDec) (l : list A),
-    {l' : list A | ssFuelOpt (S (length l)) l = Some l'}.
+Lemma minmax_neq :
+  forall (A : LinDec) (l : list A) (x y min max : A),
+    x <> y -> minmax A x y l = (min, max) -> min <> max.
 Proof.
-  intro. apply (Fix (@lengthOrder_wf A)). intros l H.
-  destruct l as [| h t]; intros.
-    simpl. exists []. trivial.
-    pose (m := min_dflt A h t). pose (r := remove_once m (h :: t)).
-      destruct (H r).
-        unfold r. apply remove_once_min_lengthOrder.
- 	      exists (min_dflt A h t :: x). rewrite ssFuelOpt_eq. fold m. fold r.
-          replace (length (h :: t)) with (S (length r)).
-            rewrite e. reflexivity.
-            unfold r. apply remove_once_In_eq.
-              apply min_In.
-Defined.
+  induction l as [| h t]; cbn; intros.
+    congruence.
+    dec.
+      destruct (LinDec_eqb_spec _ h x); subst; eauto.
+        destruct (LinDec_eqb_spec _ h y); subst; eauto.
+        eapply IHt; eauto.
+Abort.
 
-Theorem ssFuelOpt_None : forall (A : LinDec) (l : list A),
-    ssFuelOpt (S (length l)) l <> None.
-Proof.
-  unfold not; intros.
-  pose (H' := ssFuelOpt_extract A l).
-  destruct H'. rewrite e in H. inversion H.
-Defined.
-
-Definition ssFuelOpt' {A : LinDec} (l : list A) : list A :=
-    proj1_sig (ssFuelOpt_extract A l).
-
-Eval compute in ssFuelOpt' testl.
-
-Definition ssFuelOpt'' {A : LinDec} (l : list A) : list A.
-Proof.
-  case_eq (ssFuelOpt (S (length l)) l); intros.
-    exact l0.
-    apply ssFuelOpt_None in H. destruct H.
-Defined.
-
-Eval compute in ssFuelOpt'' testl.
-
-(* Selection sort using fuel recursion without options. *)
-Fixpoint ssFuel {A : LinDec} (n : nat) (l : list A) : list A :=
-match n, l with
-    | 0, _ => []
-    | _, [] => []
-    | S n', h :: t => let m := min_dflt A h t in
-        m :: ssFuel n' (remove_once m l)
-end.
-
-Eval compute in ssFuel 100 testl.
-
-(* Selection sort using well-founded recursion *)
-Definition ssWf {A : LinDec} : list A -> list A.
-Proof.
-  apply (Fix (@lengthOrder_wf A)). intros l ss.
-  destruct l as [| h t].
-    exact [].
-    pose (m := min_dflt A h t). pose (r := remove_once m (h :: t)).
-      pose (p := remove_once_min_lengthOrder A h t).
-      exact (m :: ss r p).
-Defined.
-
-Eval compute in ssWf testl.
-
-(* Selection sort using well-founded recursion and refine. *)
-Definition ssWfRef {A : LinDec} : list A -> list A.
-refine (Fix (@lengthOrder_wf A) _ (fun (l : list A) =>
+Function ss2 (A : LinDec) (l : list A) {measure length l} : list A :=
 match l with
-    | [] => fun _ => []
-    | h :: t => fun ss => let m := min_dflt A h t in
-        m :: ss (remove_once m (h :: t)) _
-end)).
-Proof. apply remove_once_min_lengthOrder. Defined.
-
-Eval compute in ssWfRef testl.
-
-(* Selection sort using Bove-Capretta *)
-Inductive ssDom {A : LinDec} : list A -> Type :=
-    | ssDomNil : ssDom []
-    | ssDomRec : forall (h : A) (t : list A),
-        ssDom (remove_once (min_dflt A h t) (h :: t)) -> ssDom (h :: t).
-
-Fixpoint ssBC' {A : LinDec} {l : list A} (p : ssDom l)
-    : list A :=
-match p with
-    | ssDomNil => []
-    | ssDomRec h t p => min_dflt A h t :: ssBC' p
+    | [] => []
+    | [x] => [x]
+    | h :: t => let (min, max) := minmax A h h t in
+        min :: ss2 A (remove_once min (remove_once max l)) ++ [max]
 end.
-
-Theorem ssDom_all : forall (A : LinDec) (l : list A), ssDom l.
 Proof.
-  intro. apply well_founded_induction_type with lengthOrder.
-    apply lengthOrder_wf.
-    intros l ss. destruct l as [| h t]; constructor.
-      apply ss. apply remove_once_min_lengthOrder.
-Defined.
-
-Definition ssBC {A : LinDec} (l : list A) : list A :=
-    ssBC' (ssDom_all A l).
-
-Eval compute in ssBC testl.
+  intros. eapply lt_trans.
+    apply remove_once_In_lt. apply remove_once_In'.
+Abort.
