Sorting/OldQuickSort.v
@@ -1,0 +1,102 @@
+Add Rec LoadPath "/home/zeimer/Code/Coq".
+
+Require Export Coq.Program.Wf.
+Require Export Recdef.
+
+Require Export Sort.
+Require Export ListLemmas.
+
+Set Implicit Arguments.
+
+Hint Unfold lt.
+Hint Resolve le_n_S filter_length.
+
+(* Quicksort using Program Fixpoint *)
+Program Fixpoint qsPF (A : LinDec) (l : list A) {measure (length l)}
+    : list A :=
+match l with
+    | [] => []
+    | h :: t => qsPF A (filter (fun x : A => leqb x h) t) ++ [h]
+             ++ qsPF A (filter (fun x : A => negb (leqb x h)) t)
+end.
+Next Obligation. simpl. auto. Qed.
+Next Obligation. simpl. auto. Qed.
+
+Eval compute in qsPF natle testl.
+
+(* Quicksort using fuel recursion. *)
+Fixpoint qsFuel' (A : LinDec) (fuel : nat) (l : list A) : list A :=
+match fuel, l with
+    | 0, _ => l
+    | _, [] => []
+    | _, [x] => [x]
+    | S fuel', h :: t =>
+        qsFuel' A fuel' (filter (fun x : A => leqb x h) t) ++ h ::
+        qsFuel' A fuel' (filter (fun x : A => negb (leqb x h)) t)
+end.
+
+Definition qsFuel (A : LinDec) (l : list A) : list A :=
+    qsFuel' A (length l) l.
+
+Eval compute in (qsFuel natle testl).
+
+(* Quicksort using well-founded recursion. *)
+Definition qsWf (A : LinDec) : list A -> list A.
+Proof.
+  apply (Fix (@lengthOrder_wf A) _).
+  intros l qsWf.
+  destruct l as [| h t].
+    exact [].
+    pose (le := qsWf (filter (fun x : A => leqb x h) t)
+        (filter_lengthOrder (fun x => leqb x h) h t)).
+    pose (gt := qsWf (filter (fun x : A => negb (leqb x h)) t)
+        (filter_lengthOrder (fun x : A => negb (leqb x h)) h t)).
+    exact (le ++ h :: gt).
+Defined.
+
+Eval compute in qsWf natle testl.
+
+(* Quicksort using wel-founded recursion and refine. *)
+Definition qsWfRef (A : LinDec) : list A -> list A.
+refine (Fix (@lengthOrder_wf A) _ (fun (l : list A) =>
+match l with
+    | [] => fun _ => []
+    | h :: t => fun qs =>
+        qs (filter (fun x : A => leqb x h) t) _ ++ h ::
+        qs (filter (fun x : A => negb (leqb x h)) t) _
+end)).
+Proof.
+  apply filter_lengthOrder.
+  apply filter_lengthOrder.
+Defined.
+
+Eval compute in qsWfRef natle testl.
+
+(* Quicksort using Bove-Capretta *)
+Inductive qsDom {A : LinDec} : list A -> Type :=
+    | qsDom0 : qsDom nil
+    | qsDom1 : forall (h : A) (t : list A),
+        qsDom (filter (fun x : A => leqb x h) t) ->
+        qsDom (filter (fun x : A => negb (leqb x h)) t) ->
+        qsDom (h :: t).
+
+Fixpoint qsBC' {A : LinDec} (l : list A) (dom : qsDom l) : list A :=
+match dom with
+    | qsDom0 => nil
+    | qsDom1 h t dom1 dom2 =>
+        qsBC' dom1 ++ h :: qsBC' dom2
+end.
+
+Theorem all_qsDom : forall (A : LinDec) (l : list A), qsDom l.
+Proof.
+  intro. apply well_founded_induction_type with lengthOrder.
+    apply lengthOrder_wf.
+    intros. destruct x as [| h t]; constructor; apply X.
+      simpl. unfold lt. apply le_n_S. apply filter_length.
+      simpl. unfold lt. apply le_n_S. apply filter_length.
+Defined.
+
+Definition qsBC (A : LinDec) (l : list A) : list A :=
+    @qsBC' A l (all_qsDom A l).
+
+Eval compute in qsBC natle testl.
