Sorting/QuicksortSpec.v
@@ -2,58 +2,14 @@ Add Rec LoadPath "/home/zeimer/Code/Coq".
 
 Require Import QuickSort.
 
+Require Import InsertionSort.
+
 Set Implicit Arguments.
 
-Theorem qsFun_In :
-  forall (A : LinDec) (x : A) (l : list A),
-    In x (qsFun A l) <-> In x l.
+Theorem qs_perm :
+  forall (A : LinDec) (l : list A), perm A l (qs A l).
 Proof.
-  split; functional induction qsFun A l; auto.
-    intros H %in_app_or. destruct (LinDec_eqb_spec _ x h); subst.
-      left. auto.
-      right. apply filter_In_app with (fun x : A=> x <=? h).
-        apply in_or_app. destruct H.
-          left. apply IHl0. assumption.
-          right. apply IHl1. inversion H; subst; intuition.
-    intro. apply in_or_app. inversion H; subst.
-      right. left. auto.
-      case_eq (x <=? h); intros.
-        left. apply IHl0, filter_In. auto.
-        right. right. apply IHl1, filter_In. rewrite H1. auto.
-Qed.
-
-Theorem qsFun_sorted :
-  forall (A : LinDec) (l : list A), sorted A (qsFun A l).
-Proof.
-  intros. functional induction qsFun A l.
-    constructor.
-    apply sorted_app_all.
-      assumption.
-      apply sorted_cons.
-        intros. rewrite qsFun_In, filter_In in H. destruct H.
-          destruct (leqb_spec x h).
-            inversion H0.
-            apply LinDec_not_leq. assumption.
-          assumption.
-      intros. rewrite qsFun_In, filter_In in H. destruct H.
-        destruct (leqb_spec x h); intuition.
-Qed.
-
-Hint Resolve filter_lengthOrder.
-
-Theorem qsFun_perm :
-  forall (A : LinDec) (l : list A), perm A l (qsFun A l).
-Proof.
-  unfold perm. intros A l x. generalize dependent l.
-  apply (well_founded_ind (@lengthOrder_wf A)
-    (fun l : list A => count A x l = count A x (qsFun A l))).
-  destruct x0 as [| h t]; intro IH.
-    compute. reflexivity.
-    rewrite qsFun_equation. rewrite count_app. simpl. dec.
-      rewrite <- !IH, (count_filter A h h) by auto. omega.
-      erewrite <- !IH, count_filter; auto.
-Restart.
-  intros A l. functional induction qsFun A l.
+  intros A l. functional induction qs A l.
     auto.
     apply perm_symm. eapply perm_trans.
       apply perm_front.
@@ -61,9 +17,97 @@ Restart.
         rewrite count_app, <- IHl0, <- IHl1, <- count_filter. auto.
 Qed.
 
-Instance Sort_qsFun : Sort :=
+Theorem qs_In :
+  forall (A : LinDec) (x : A) (l : list A),
+    In x (qs A l) <-> In x l.
+Proof.
+  intros. rewrite !count_In, <- qs_perm. reflexivity.
+Qed.
+
+Theorem qs_sorted :
+  forall (A : LinDec) (l : list A), sorted A (qs A l).
+Proof.
+  intros. functional induction qs A l.
+    constructor.
+    apply sorted_app_all.
+      assumption.
+      apply sorted_cons.
+        intros. rewrite qs_In, filter_In in H. destruct H.
+          destruct (leqb_spec x h).
+            inversion H0.
+            apply LinDec_not_leq. assumption.
+          assumption.
+      intros. rewrite qs_In, filter_In in H. destruct H.
+        destruct (leqb_spec x h); intuition.
+Qed.
+
+Instance Sort_qs : Sort :=
 {
-    sort := qsFun;
-    sort_sorted := qsFun_sorted;
-    sort_perm := qsFun_perm;
+    sort := qs;
+    sort_sorted := qs_sorted;
+    sort_perm := qs_perm;
+}.
+
+Theorem qs2_is_qs :
+  forall (A : LinDec) (l : list A), qs2 A l = qs A l.
+Proof.
+  intros. functional induction qs2 A l.
+    compute. trivial.
+    rewrite qs_equation. rewrite bifilter_spec in e0.
+      inversion e0. rewrite H0, H1. congruence.
+Qed.
+
+Instance Sort_qs2 : Sort :=
+{
+    sort := qs2
+}.
+Proof.
+  all: intros; rewrite qs2_is_qs.
+    apply (@sort_sorted Sort_qs).
+    apply (@sort_perm Sort_qs).
+Defined.
+
+Theorem hqs_perm :
+  forall (n : nat) (A : LinDec) (l : list A), perm A l (hqs n A l).
+Proof.
+  intros. functional induction hqs n A l; trivial.
+    apply (@sort_perm Sort_insertionSort).
+    apply perm_symm. eapply perm_trans.
+      apply perm_front.
+      apply perm_cons. unfold perm in *. intro.
+        rewrite count_app, <- IHl0, <- IHl1.
+        rewrite bifilter_spec in e1; inversion_clear e1.
+        rewrite <- count_filter. auto.
+Qed.
+
+Theorem hqs_In :
+  forall (n : nat) (A : LinDec) (x : A) (l : list A),
+    In x (hqs n A l) <-> In x l.
+Proof.
+  intros. rewrite !count_In, <- hqs_perm. reflexivity.
+Qed.
+
+Theorem hqs_sorted :
+  forall (n : nat) (A : LinDec) (l : list A), sorted A (hqs n A l).
+Proof.
+  intros. functional induction hqs n A l.
+    apply (@sort_sorted Sort_insertionSort).
+    constructor.
+    rewrite bifilter_spec in e1; inversion e1; subst. apply sorted_app_all.
+      assumption.
+       apply sorted_cons.
+        intros. rewrite hqs_In, filter_In in H. destruct H.
+          destruct (leqb_spec x h).
+            inversion H0.
+            apply LinDec_not_leq. assumption.
+          assumption.
+      intros. rewrite hqs_In, filter_In in H. destruct H.
+        destruct (leqb_spec x h); intuition.
+Qed.
+
+Instance Sort_hqs (n : nat) : Sort :=
+{
+    sort := hqs n;
+    sort_sorted := hqs_sorted n;
+    sort_perm := hqs_perm n;
 }.
