Sorting/SelectionSortSpec.v
@@ -4,74 +4,44 @@ Require Import SelectionSort.
 
 Set Implicit Arguments.
 
-Lemma ssFun_In :
+Lemma ss_In :
   forall (A : LinDec) (x : A) (l : list A),
-    In x l -> In x (ssFun A l).
+    In x (ss A l) <-> In x l.
 Proof.
-  intros A x. apply (well_founded_ind (@lengthOrder_wf A)
-    (fun l : list A => In x l -> In x (ssFun A l))).
-  destruct x0 as [| h t]; intro IH; inversion 1; subst;
-  rewrite ssFun_equation.
-    simpl. dec. right. apply IH.
-      apply remove_once_cons. assumption.
-      constructor. reflexivity.
-    simpl. dec.
-      right. apply IH.
-        red; simpl; omega.
-        assumption.
+  split; functional induction ss A l; intros; auto.
+    destruct H; subst.
+      apply min_In.
+      destruct (min_split A h t) as [l1 [l2 [H1 H2]]].
+        rewrite <- H2 in *.
+          pose (wut := IHl0 H). rewrite H1. apply in_or_app.
+            destruct (@in_app_or _ _ _ _ wut); [left | do 2 right]; auto.
+    cbn in *. destruct H; dec.
+      right. apply IHl0. left. auto.
       destruct (LinDec_eqb_spec A x (min_dflt A h t)).
         left. auto.
-        right. apply IH.
-          apply remove_once_cons. assumption.
+        right. apply IHl0.
           simpl. right. apply remove_once_In; auto.
 Qed.
 
-Lemma ssFun_In_conv :
-  forall (A : LinDec) (x : A) (l : list A),
-    In x (ssFun A l) -> In x l.
+Theorem ss_sorted :
+  forall (A : LinDec) (l : list A), sorted A (ss A l).
 Proof.
-  intros A x. apply (well_founded_ind (@lengthOrder_wf A)
-    (fun l : list A => In x (ssFun A l) -> In x l)).
-  destruct x0 as [| h t]; intro IH.
-    inversion 1.
-    rewrite ssFun_equation. inversion 1.
-      rewrite <- H0. apply min_In.
-      destruct (min_split A h t) as [l1 [l2 [H1 H2]]].
-        rewrite <- H2 in *. assert (lengthOrder (l1 ++ l2) (h :: t)).
-          rewrite H2. apply remove_once_min_lengthOrder.
-          pose (wut := IH _ H3 H0). rewrite H1. apply in_or_app.
-            destruct (@in_app_or _ _ _ _ wut); [left | do 2 right]; auto.
-Qed.
-
-Theorem ssFun_sorted :
-  forall (A : LinDec) (l : list A), sorted A (ssFun A l).
-Proof.
-  intros. functional induction ssFun A l.
+  intros. functional induction ss A l.
     constructor.
-    case_eq (ssFun A (remove_once (min_dflt A h t) (h :: t))); intros.
+    case_eq (ss A (remove_once (min_dflt A h t) (h :: t))); intros.
       auto.
       constructor.
-        assert (In c (ssFun A (remove_once (min_dflt A h t) (h :: t)))).
+        assert (In c (ss A (remove_once (min_dflt A h t) (h :: t)))).
           rewrite H. left. reflexivity.
-          apply ssFun_In_conv in H0. apply min_spec.
+          rewrite ss_In in H0. apply min_spec.
           apply remove_once_In_conv in H0. assumption.
         rewrite <- H. assumption.
 Qed.
 
-Theorem ssFun_perm :
-  forall (A : LinDec) (l : list A), perm A l (ssFun A l).
+Theorem ss_perm :
+  forall (A : LinDec) (l : list A), perm A l (ss A l).
 Proof.
-  intro. apply well_founded_ind with lengthOrder.
-    apply lengthOrder_wf.
-    destruct x as [| h t]; intro IH; rewrite ssFun_equation.
-      apply perm_refl.
-      destruct (min_split A h t) as [l1 [l2 [H H']]].
-      rewrite <- H', H. eapply perm_trans.
-        apply perm_front.
-        apply perm_cons. apply IH. rewrite H. unfold lengthOrder.
-          rewrite 2 app_length. simpl. omega.
-Restart.
-  intros. functional induction ssFun A l.
+  intros. functional induction ss A l.
     auto.
     destruct (min_split A h t) as [l1 [l2 [H H']]].
       rewrite <- H', H in *. eapply perm_trans.
@@ -79,9 +49,9 @@ Restart.
         apply perm_cons. apply IHl0.
 Qed.
 
-Instance Sort_ssFun : Sort :=
+Instance Sort_ss : Sort :=
 {
-    sort := ssFun;
-    sort_sorted := ssFun_sorted;
-    sort_perm := ssFun_perm
+    sort := ss;
+    sort_sorted := ss_sorted;
+    sort_perm := ss_perm
 }.
