Sorting/Test.v
@@ -9,18 +9,14 @@ Require Import HybridSorts.
 
 Set Implicit Arguments.
 
-Time Eval compute in insertionSort natle testl.
-Time Eval compute in ssFun natle testl.
-Time Eval compute in qsFun natle testl.
-
 Fixpoint cycle {A : Type} (n : nat) (l : list A) : list A :=
 match n with
     | 0 => []
     | S n' => l ++ cycle n' l
 end.
 
-Extraction Language Haskell.
-Extraction hms2.
+(*Time Compute hqs 128 natle (cycle 100 testl).
+Time Compute hms 128 natle (cycle 100 testl).*)
 
 (*Time Compute hms2 128 natle (cycle 100 testl).
 Time Compute ms natle (cycle 100 testl).
@@ -28,7 +24,6 @@ Time Compute ms2 natle (cycle 100 testl).
 Time Compute hms 128 natle (cycle 100 testl).
 
 Time Compute qs natle (cycle 500 testl).
-Time Compute hqs natle 1024 (cycle 500 testl).
 Time Compute insertionSort natle (cycle 500 testl).
 Time Compute ssFun natle (cycle 200 testl).
 Time Compute qs2 natle (cycle 200 testl).*)
